\documentclass{article}
\usepackage{amsmath,amssymb}
\usepackage{mathtools}
\usepackage{amsfonts}
\usepackage{amssymb}
\usepackage{tikz}

\DeclarePairedDelimiter{\ceil}{\lceil}{\rceil}
\newcounter{question}
\setcounter{question}{0}
\begin{document}

\newcommand\Que[1]{%
   \leavevmode\par
   \stepcounter{question}
   \noindent
   \thequestion. Q --- #1\par}

\newcommand\Ans[2][]{%
    \leavevmode\par\noindent
   {\leftskip37pt
    A --- \textbf{#1}#2\par}}

\Que{
    Find the general solution of the recurrence equation\\
    $g_{n+2} = 3g_{n+1}-2g_n$.
}
\Ans{
    The recurrence can be written as a homogenous
    equation, \\
    $g_{n+2} - 3g_{n+1} + 2g_n=0$. On summating:
    \begin{equation}
        \sum_{n=0}^\infty {g_{n+2}} 
        - 3\sum_{n=0}^\infty {g_{n+1}} 
        + 2\sum_{n=0}^\infty {g_n}=0
    \end{equation}

    \begin{align*}
        \sum_{n=0}^\infty {g_{n+1}x^n} & = 
        g_1+g_2x+g_3x^2+g_4x^3+\cdots\\
        x\sum_{n=0}^\infty {g_{n+1}x^n} & = 
        g_1x+g_2x^2+g_3x^3+g_4x^4+\cdots\\
        & = f(x) - g_0\\
        \therefore
        \sum_{n=0}^\infty {g_{n+1}x^n} & = 
        \frac{f(x) - g_0}{x}
    \end{align*}

    \boxed{
        r_n = \frac{g_0-g_1}{2} (-1)^n
        + \frac{g_0+g_1}{2}
    }
}

\Que{
    Find the general solution of the recurrence equation\\
    $g_{n+2} = 3g_{n+1}-2g_n$.
}
\Ans{
    The recurrence can be written as a homogenous
    equation, \\
}
\end{document}
